



Kinematics

1-D Kinematics

Position $x(t)$

Special Case: Constant Acceleration

Velocity $v(t) = \frac{d}{dt}x(t)$

$a = \text{constant}$

$v(t) = v_0 + at$

Acceleration $a(t) = \frac{d}{dt}v(t)$

$x(t) = x_0 + v_0t + \frac{1}{2}at^2$

$v^2 = v_0^2 + 2a(x - x_0)$

3-D Kinematics

$\mathbf{r}(t) = x(t)\mathbf{i} + y(t)\mathbf{j} + z(t)\mathbf{k}$

Special Case: Projectile Motion

$\mathbf{v}(t) = \frac{d}{dt}\mathbf{r}(t) = \frac{dx}{dt}\mathbf{i} + \frac{dy}{dt}\mathbf{j} + \frac{dz}{dt}\mathbf{k}$
 $= v_x(t)\mathbf{i} + v_y(t)\mathbf{j} + v_z(t)\mathbf{k}$

$a_x = 0$ $a_y = -g$
 $v_x(t) = v_{0x}$ $v_y(t) = v_{0y} - gt$
 $x(t) = x_0 + v_{0x}t$ $y(t) = y_0 + v_{0y}t - \frac{1}{2}gt^2$

$\mathbf{a}(t) = \frac{d}{dt}\mathbf{v}(t) = \frac{d^2x}{dt^2}\mathbf{i} + \frac{d^2y}{dt^2}\mathbf{j} + \frac{d^2z}{dt^2}\mathbf{k}$
 $= a_x(t)\mathbf{i} + a_y(t)\mathbf{j} + a_z(t)\mathbf{k}$

Galilean Transformations

$\mathbf{v} = \mathbf{w} + \mathbf{v}_F$

$\mathbf{r}(t) = \mathbf{r}_0 + \int_0^t \mathbf{v}(t')dt'$

$\mathbf{v}(t) = \mathbf{v}_0 + \int_0^t \mathbf{a}(t')dt'$

\mathbf{v} : Velocity in stationary frame

\mathbf{w} : Velocity in moving frame

\mathbf{v}_F : Velocity of moving frame

Circular Motion

Motion on a Circle of Radius R

$\mathbf{r}(t) = R \cos(\theta(t))\mathbf{i} + R \sin(\theta(t))\mathbf{j}$

Angular Position $\theta(t)$

Angular Velocity $\omega(t) = \frac{d}{dt}\theta(t)$

Angular Acceleration $\alpha(t) = \frac{d}{dt}\omega(t)$

Tangential Velocity $v_t = \omega R$

Tangential Acceleration $a_t = \alpha R$

Centripetal Acceleration $a_c = \omega^2 R = \frac{v_t^2}{R}$

Special Cases:

Uniform Circular Motion (Constant ω)

T : Period – time for one cycle

f : Frequency – cycles per second

$\alpha = 0 \implies a_t = 0$ $\omega = \text{constant}$

$\omega = \frac{2\pi}{T} = 2\pi f$ $v_t = \omega R$

Constant Angular Acceleration (Constant α)

$\alpha = \text{constant}$ $\omega(t) = \omega_0 + \alpha t$

$\theta(t) = \theta_0 + \omega_0 t + \frac{1}{2}\alpha t^2$ $\omega^2 = \omega_0^2 + 2\alpha(\theta - \theta_0)$

Dynamics

Newton's Three Laws

$$\sum \mathbf{F} = \mathbf{0}$$
$$\Rightarrow \mathbf{v} = \text{constant}$$

Objects in motion tend to stay in motion unless acted upon by an external force.

$$\sum \mathbf{F} = m\mathbf{a}$$

The sum of all the forces acting on an object equals the object's mass times its acceleration.

$$\mathbf{F}_{12} = -\mathbf{F}_{21}$$

For every action there is an equal and opposite reaction.

Common Forces

Normal Force $0 \leq N \leq \infty$

The normal force exerts enough force to keep an object from traveling through another.

Static Friction $0 \leq F_S \leq \mu_s N$

Static friction exerts enough force to keep an object from sliding until the force required is greater than $\mu_s N$

Kinetic Friction $F_K = \mu_k N$

Kinetic friction applies to a sliding object on a surface with friction and opposes the direction of motion.

Spring Force $F_E = -k(x - x_0)$

Elastic forces, such as for a spring, act in the direction of the equilibrium position x_0 and are linearly proportional to the displacement from equilibrium $x - x_0$.

Circular Dynamics

For Circular Motion:

$$a_c = \omega^2 R = \frac{v_t^2}{R} \Rightarrow \sum F = F_c = m\omega^2 R = \frac{mv_t^2}{R}$$

The sum of the forces (net force) must equal F_c , the centripetal force, to have circular motion. The centripetal force and acceleration point towards the center of the circle.

Conservation Laws

Work & Kinetic Energy

Work – Variable Force	$\int_{\mathbf{r}_1}^{\mathbf{r}_2} \mathbf{F} \cdot d\mathbf{r}$	Work-Energy Theorem
Work – Constant Force	$\mathbf{F} \cdot \mathbf{d} = Fd \cos \theta$	$\Delta K = K_f - K_i = W_{net}$
Kinetic Energy	$K = \frac{1}{2}mv^2$	The change in kinetic energy of a system is equal to the net work done.
Power	$P = \frac{dW}{dt} = \mathbf{F} \cdot \mathbf{v}$	
$W_{net} > 0$: Energy is transferred into the system		
$W_{net} < 0$: Energy is transferred out of the system		

Potential Energy

Conservative Force	$\oint \mathbf{F}_c \cdot d\mathbf{r} = 0$	Generalized Work-Energy Theorem
Potential Energy	$\Delta U = - \int_{\mathbf{r}_1}^{\mathbf{r}_2} \mathbf{F}_c \cdot d\mathbf{r}$	
		$\Delta E = \Delta K + \Delta U = W_{ext}$
Force – Potential	$F_c(x) = -\frac{d}{dx}U(x)$	The change in mechanical energy of a system is equal to the net work done by external (non-conservative) forces.
Gravitational Potential	$U_g(y) = mgy + U_0$	
Elastic Potential	$U_e(x) = \frac{1}{2}k(x - x_0)^2$	
For an isolated system $W_{ext} = 0$ and $\Delta E = 0 \implies K_i + U_i = K_f + U_f$		

Linear Momentum

		Inelastic Collisions	Elastic Collisions
Momentum	$\mathbf{p} = m\mathbf{v}$	$\sum \mathbf{p}_i = \sum \mathbf{p}_f$	$\sum \mathbf{p}_i = \sum \mathbf{p}_f$
Impulse	$\mathbf{J} = \Delta \mathbf{p} = \int_{t_1}^{t_2} \mathbf{F}(t)dt$		$K_i = K_f$
Newton's Second Law	$\mathbf{F} = \frac{d}{dt}\mathbf{p}$	1D elastic collision with $v_{2i} = 0$:	
Conservation of Momentum	$\sum \mathbf{p}_i = \sum \mathbf{p}_f$	$v_{1f} = \frac{m_1 - m_2}{m_1 + m_2}v_{1i}$	$v_{2f} = \frac{2m_1}{m_1 + m_2}v_{1i}$

Angular Momentum

Angular Momentum Single Particle	$\mathbf{L} = \mathbf{r} \times \mathbf{p}$	Conservation of Angular Momentum:
Angular Momentum Rigid Body	$\mathbf{L} = I\boldsymbol{\omega}$	$\mathbf{L}_i = \mathbf{L}_f$
Newton's Second Law	$\boldsymbol{\tau} = \frac{d}{dt}\mathbf{L}$	if
		$\boldsymbol{\tau}_{ext} = \frac{d}{dt}\mathbf{L} = \mathbf{0}$

Rigid Body Motion

Center of Mass

Center of Mass	$\mathbf{r}_{CM} = \frac{\sum_i m_i \mathbf{r}_i}{M}$ $M = \sum_i m_i$	The center of mass represents the point about which a rigid body behaves as a point mass with total mass M .
Linear Momentum	$\mathbf{p} = M\mathbf{v}_{CM}$	The total linear momentum of a rigid body is the total mass times the velocity of the center of mass.
Newton's 2nd Law	$\sum \mathbf{F} = M\mathbf{a}_{CM}$	The sum of all forces causes a linear acceleration of the center of mass.

Moment of Inertia

Moment of Inertia	$I = \sum_i m_i r_i^2$	The moment of inertia represent how a rigid body resists rotation about its center of mass.
Torque	$\boldsymbol{\tau} = \mathbf{r} \times \mathbf{F}$ $\tau = rF \sin \phi$	A force applied at a distance from a rotation point induces a torque about the axis of rotation.
Newton's 2nd Law	$\sum_i \tau_i = I\alpha$	The sum of all torques causes an angular acceleration about the center of mass or rotation point.

Energy of a Rigid Body

Translational Kinetic Energy	$K_t = \frac{1}{2} M v_{CM}^2$	Rolling Without Slipping:
Rotational Kinetic Energy	$K_r = \frac{1}{2} I \omega^2$	$v_{CM} = R\omega \quad a_{CM} = R\alpha$
Total Kinetic Energy	$K = K_t + K_r$	$K = K_t + K_r = \frac{1}{2} v_{CM}^2 \left(M + \frac{I}{R^2} \right)$

Waves and Oscillations

Simple Harmonic Oscillator

General Solution		Properties	
Displacement	$x(t) = A \cos(\omega_0 t + \phi)$	Period	$T = \frac{2\pi}{\omega_0}$
Velocity	$v(t) = -A\omega_0 \sin(\omega_0 t + \phi)$	Frequency	$f = \frac{\omega_0}{2\pi} = \frac{1}{T}$
Acceleration	$a(t) = -A\omega_0^2 \cos(\omega_0 t + \phi)$	Restoring Force	$F(t) = -Cx(t)$
Resonance Frequency		Kinetic Energy	$K(t) = \frac{A^2\omega_0^2 m}{2} \sin^2(\omega_0 t + \phi)$
Mass-Spring	$\omega_0 = \sqrt{\frac{k}{m}}$	Potential Energy	$U(t) = \frac{A^2\omega_0^2 m}{2} \cos^2(\omega_0 t + \phi)$
Pendulum	$\omega_0 = \sqrt{\frac{g}{L}}$		
Damped Oscillator: $\omega_d = \sqrt{ \alpha^2 - \omega_0^2 }$			
Overdamped: $\alpha > \omega_0$		Underdamped: $\alpha < \omega_0$	
$x(t) = e^{-\alpha t} [A \cosh(\omega_d t) + B \sinh(\omega_d t)]$		$x(t) = e^{-\alpha t} [A \cos(\omega_d t) + B \sin(\omega_d t)]$	

Waves

General Properties		Traveling Waves	
Wavespeed	c	D'Alembert Solution	$y(x, t) = f(x - ct) + g(x + ct)$
Wavelength	$\lambda = \frac{c}{f}$	Sinusoidal Solution	$y(x, t) = A \cos(kx \pm \omega t + \phi)$
Wavenumber	$k = \frac{2\pi}{\lambda} = \frac{\omega}{c}$	Standing Waves	
		Fixed-Fixed String	$y_n(x, t) = A_n \sin(k_n x) \cos(\omega_n t + \phi)$
			$k_n = \frac{n\pi}{L}, \quad n = 1, 2, 3, \dots$

Acoustics

1D Plane Wave		Pipe Resonance Frequencies	
Spherical Wave	$p(r, t) = \frac{A \cos(kx - \omega t + \phi)}{r}$	Open-Open	$p_n(x, t) = A_n \sin(k_n x) \cos(\omega_n t)$ $k_n = \frac{n\pi}{L}, \quad n = 1, 2, 3, \dots$
Sound Intensity	$I = \frac{P}{S}$	Closed-Closed	$p_n(x, t) = A_n \cos(k_n x) \cos(\omega_n t)$ $k_n = \frac{n\pi}{L}, \quad n = 1, 2, 3, \dots$
(dB)	$L = 10 \log_{10} I/I_0$	Open-Closed	$p_n(x, t) = A_n \cos(k_n x) \cos(\omega_n t)$ $k_n = \frac{n\pi}{4L}, \quad n = 1, 3, 5, \dots$
	$I_0 = 1 \text{ pW}$		